src/Init/Data/Char/Ordinal.lean
@@ -130,7 +130,7 @@ theorem ofOrdinal_ordinal {c : Char} : Char.ofOrdinal c.ordinal = c := by
   simp only [val_ofOrdinal, coe_ordinal, UInt32.ofNatLT_add]
   split
   · grind [UInt32.lt_iff_toNat_lt, UInt32.ofNatLT_toNat]
-  · rw [dif_neg]
+  · rw [dite_eq_right]
     · simp only [← UInt32.toNat_inj, UInt32.toNat_add, UInt32.toNat_ofNatLT, Nat.reducePow]
       grind [UInt32.toNat_lt, UInt32.lt_iff_toNat_lt]
     · grind [UInt32.lt_iff_toNat_lt]
@@ -140,9 +140,9 @@ theorem ordinal_ofOrdinal {f : Fin Char.numCodePoints} : (Char.ofOrdinal f).ordi
   ext
   simp [coe_ordinal, val_ofOrdinal]
   split
-  · rw [if_pos, UInt32.toNat_ofNatLT]
+  · rw [ite_eq_left, UInt32.toNat_ofNatLT]
     simpa [UInt32.lt_iff_toNat_lt]
-  · rw [if_neg, UInt32.toNat_add, UInt32.toNat_ofNatLT, UInt32.toNat_ofNatLT, Nat.mod_eq_of_lt,
+  · rw [ite_eq_right, UInt32.toNat_add, UInt32.toNat_ofNatLT, UInt32.toNat_ofNatLT, Nat.mod_eq_of_lt,
       Nat.add_sub_cancel]
     · grind
     · simp only [UInt32.lt_iff_toNat_lt, UInt32.toNat_add, UInt32.toNat_ofNatLT, Nat.reducePow,
@@ -188,7 +188,7 @@ theorem ofOrdinal_le_of_le {f g : Fin Char.numCodePoints} (h : f ≤ g) :
     · simp only [UInt32.toNat_add, UInt32.toNat_ofNatLT, Nat.reducePow]
       grind
   · simp only [UInt32.toNat_add, UInt32.toNat_ofNatLT, Nat.reducePow]
-    rw [dif_neg (by grind)]
+    rw [dite_eq_right (by grind)]
     simp only [UInt32.toNat_add, UInt32.toNat_ofNatLT, Nat.reducePow]
     grind
 
@@ -233,7 +233,7 @@ theorem succ?_eq {c : Char} : c.succ? = (c.ordinal.addNat? 1).map Char.ofOrdinal
       · rename_i h1 h2 _ h3
         simp only [← UInt32.toNat_inj, UInt32.lt_iff_toNat_lt, UInt32.toNat_ofNat] at h1 h2 h3
         omega
-      · rw [dif_neg]
+      · rw [dite_eq_right]
         · simp only [← UInt32.toNat_inj, UInt32.toNat_add, UInt32.reduceToNat, Nat.reducePow,
             UInt32.toNat_ofNatLT, Nat.mod_add_mod]
           grind [UInt32.lt_iff_toNat_lt, UInt32.toNat_inj]
